correctness/RegexCorrectness/Backtracker/Traversal/Lemmas.lean
@@ -13,20 +13,20 @@ variable {nfa : NFA} {wf : nfa.WellFormed} {startIdx maxIdx : Nat} {bit₀ bit :
   {visited : BitMatrix nfa.nodes.size (maxIdx + 1 - startIdx)} {stack : List (StackEntry HistoryStrategy nfa startIdx maxIdx)}
 
 theorem mem_or_path_of_mem_of_none {result} (hres : captureNextAux HistoryStrategy nfa wf startIdx maxIdx visited [⟨HistoryStrategy.empty, ⟨nfa.start, wf.start_lt⟩, bit⟩] = result)
-  (isNone : result.1 = .none) (v : bit.Valid) :
-  VisitedInv wf bit visited result.2 :=
-  visited_inv_of_none hres isNone VisitedInv.rfl (StackInv.intro v)
+  (isNone : result.1 = .none) (reaches : bit₀.Reaches bit) :
+  VisitedInv wf bit₀ bit reaches visited result.2 :=
+  visited_inv_of_none hres isNone (VisitedInv.rfl reaches) (StackInv.intro reaches.validR)
 
 theorem PathClosure.preserves {result} (hres : captureNextAux HistoryStrategy nfa wf startIdx maxIdx visited [⟨HistoryStrategy.empty, ⟨nfa.start, wf.start_lt⟩, bit⟩] = result)
-  (isNone : result.1 = .none) (reaches₀ : bit₀.Reaches bit) (cls : PathClosure bit₀ visited) :
+  (isNone : result.1 = .none) (reaches : bit₀.Reaches bit) (cls : PathClosure bit₀ visited) :
   PathClosure bit₀ result.2 := by
   have cinv : ClosureInv bit₀ visited [⟨HistoryStrategy.empty, ⟨nfa.start, wf.start_lt⟩, bit⟩] := by
     intro state bit state' bit' update reaches hmem step
     exact .inl (cls state bit state' bit' (List.ofOption update) reaches hmem (.last step))
-  exact path_closure hres isNone reaches₀ cinv (StackInv.intro reaches₀.validR)
+  exact path_closure hres isNone reaches cinv (StackInv.intro reaches.validR)
 
 theorem mem_of_path_of_none {result} (hres : captureNextAux HistoryStrategy nfa wf startIdx maxIdx visited [⟨HistoryStrategy.empty, ⟨nfa.start, wf.start_lt⟩, bit⟩] = result)
-  (isNone : result.1 = .none) (reaches₀ : bit₀.Reaches bit) (cls : PathClosure bit₀ visited)
+  (isNone : result.1 = .none) (reaches : bit₀.Reaches bit) (cls : PathClosure bit₀ visited)
   (bit' : BoundedIterator startIdx maxIdx) (state : Fin nfa.nodes.size) (update : List (Nat × Pos)) (path : Path nfa wf bit.it bit'.it state update) :
   result.2.get state bit'.index := by
   have mem_start : result.2.get ⟨nfa.start, wf.start_lt⟩ bit.index := hres ▸ mem_stack_top ⟨HistoryStrategy.empty, ⟨nfa.start, wf.start_lt⟩, bit⟩ [] rfl
@@ -35,20 +35,20 @@ theorem mem_of_path_of_none {result} (hres : captureNextAux HistoryStrategy nfa 
     have eq : bit' = bit := BoundedIterator.ext eqit
     simpa [eq, ←eqstate] using mem_start
   | .inr path =>
-    have cls' : PathClosure bit₀ result.2 := cls.preserves hres isNone reaches₀
-    exact cls' ⟨nfa.start, wf.start_lt⟩ bit state bit' update reaches₀ mem_start path
+    have cls' : PathClosure bit₀ result.2 := cls.preserves hres isNone reaches
+    exact cls' ⟨nfa.start, wf.start_lt⟩ bit state bit' update reaches mem_start path
 
 theorem mem_iff_mem_or_path_of_none {result} (hres : captureNextAux HistoryStrategy nfa wf startIdx maxIdx visited [⟨HistoryStrategy.empty, ⟨nfa.start, wf.start_lt⟩, bit⟩] = result)
-  (isNone : result.1 = .none) (reaches₀ : bit₀.Reaches bit) (cls : PathClosure bit₀ visited)
-  (bit' : BoundedIterator startIdx maxIdx) (state : Fin nfa.nodes.size) (reaches : bit.Reaches bit') :
+  (isNone : result.1 = .none) (reaches : bit₀.Reaches bit) (cls : PathClosure bit₀ visited)
+  (bit' : BoundedIterator startIdx maxIdx) (state : Fin nfa.nodes.size) (reaches' : bit₀.Reaches bit') :
   result.2.get state bit'.index ↔ visited.get state bit'.index ∨ ∃ update, Path nfa wf bit.it bit'.it state update := by
   apply Iff.intro
   . intro mem
-    exact mem_or_path_of_mem_of_none hres isNone reaches₀.validR state bit' reaches mem
+    exact mem_or_path_of_mem_of_none hres isNone reaches state bit' reaches' mem
   . intro h
     match h with
     | .inl mem => exact hres ▸ mem_of_mem_visited mem
-    | .inr ⟨update, path⟩ => exact mem_of_path_of_none hres isNone reaches₀ cls bit' state update path
+    | .inr ⟨update, path⟩ => exact mem_of_path_of_none hres isNone reaches cls bit' state update path
 
 end captureNextAux
 
@@ -83,42 +83,61 @@ structure Inv (wf : nfa.WellFormed) (bit₀ bit : BoundedIterator startIdx maxId
 
 namespace Inv
 
+theorem mem_iff_of_aux_none {result} (haux : captureNextAux HistoryStrategy nfa wf startIdx maxIdx visited [⟨HistoryStrategy.empty, ⟨nfa.start, wf.start_lt⟩, bit⟩] = result)
+  (isNone : result.1 = .none) (reaches : bit₀.Reaches bit) (inv : Inv wf bit₀ bit visited)
+  (state' : Fin nfa.nodes.size) (bit' : BoundedIterator startIdx maxIdx) (reaches' : bit₀.Reaches bit') :
+  result.2.get state' bit'.index ↔
+    (∃ (bitPrev : BoundedIterator startIdx maxIdx) (update : List (Nat × Pos)), bitPrev.BetweenE bit₀ bit ∧ Path nfa wf bitPrev.it bit'.it state' update) ∨
+      ∃ (update : List (Nat × Pos)), Path nfa wf bit.it bit'.it state' update := by
+  rw [captureNextAux.mem_iff_mem_or_path_of_none haux isNone reaches inv.closure bit' state' reaches']
+  rw [inv.mem_iff_path state' bit' reaches']
+
 theorem preservesAux {result} (haux : captureNextAux HistoryStrategy nfa wf startIdx maxIdx visited [⟨HistoryStrategy.empty, ⟨nfa.start, wf.start_lt⟩, bit⟩] = result)
   (isNone : result.1 = .none) (hnext : bit.hasNext) (reaches : bit₀.Reaches bit)
   (inv : Inv wf bit₀ bit visited) :
   Inv wf bit₀ (bit.next hnext) result.2 := by
   refine ⟨inv.closure.preserves haux isNone reaches, ?_⟩
   intro state' bit' reaches'
-  rw [captureNextAux.mem_iff_mem_or_path_of_none haux isNone reaches inv.closure bit' state' sorry]
-  rw [inv.mem_iff_path state' bit' reaches']
+  rw [inv.mem_iff_of_aux_none haux isNone reaches state' bit' reaches']
   simp only [exists_and_left, BoundedIterator.BetweenE.next_iff reaches.validR hnext, or_and_right,
     exists_or, existsAndEq, reaches, and_self, true_and]
 
 end Inv
 
-def MemIffPathI (wf : nfa.WellFormed) (bit₀ : BoundedIterator startIdx maxIdx) (visited : BitMatrix nfa.nodes.size (maxIdx + 1 - startIdx)) : Prop :=
+def MemIffPath (wf : nfa.WellFormed) (bit₀ : BoundedIterator startIdx maxIdx) (visited : BitMatrix nfa.nodes.size (maxIdx + 1 - startIdx)) : Prop :=
   ∀ (state' : Fin nfa.nodes.size) (bit' : BoundedIterator startIdx maxIdx),
     bit₀.Reaches bit' →
-    (visited.get state' bit'.index ↔ ∃ (bitPrev : BoundedIterator startIdx maxIdx) (update : List (Nat × Pos)), bitPrev.BetweenE bit₀ bit' ∧ Path nfa wf bitPrev.it bit'.it state' update)
+    (visited.get state' bit'.index ↔ ∃ (bit : BoundedIterator startIdx maxIdx) (update : List (Nat × Pos)), bit₀.Reaches bit ∧ Path nfa wf bit.it bit'.it state' update)
 
 theorem mem_iff_path_of_none {result} (hres : go HistoryStrategy nfa wf startIdx maxIdx bit visited = result)
-  (isNone : result.1 = .none) (inv : Inv wf bit₀ bit visited) :
-  MemIffPathI wf bit₀ result.2 := by
+  (isNone : result.1 = .none) (reaches : bit₀.Reaches bit) (inv : Inv wf bit₀ bit visited) :
+  MemIffPath wf bit₀ result.2 := by
   induction bit, visited using captureNext.go.induct' HistoryStrategy nfa wf startIdx maxIdx with
   | found bit visited update visited' haux =>
     rw [captureNext.go_found haux] at hres
     simp [←hres] at isNone
   | not_found_next bit visited visited' haux hnext ih =>
     rw [captureNext.go_not_found_next haux hnext] at hres
-    exact ih hres (inv.preservesAux haux rfl hnext sorry)
+    exact ih hres (reaches.next' hnext) (inv.preservesAux haux rfl hnext reaches)
   | not_found_end bit visited visited' haux hnext =>
     rw [captureNext.go_not_found_end haux hnext] at hres
-    have eq : bit = bit₀.last := sorry
-    subst bit
 
     intro state' bit' reaches'
-    have := captureNextAux.mem_iff_mem_or_path_of_none haux rfl sorry inv.closure bit' state' -- ???
-    sorry
+    rw [←hres, inv.mem_iff_of_aux_none haux rfl reaches state' bit' reaches']
+    apply Iff.intro
+    . intro h
+      match h with
+      | .inl ⟨bitPrev, update, between, path⟩ => exact ⟨bitPrev, update, between.2.1, path⟩
+      | .inr ⟨update, path⟩ => exact ⟨bit, update, reaches, path⟩
+    . have eq : bit = bit₀.toEnd := by
+        simp [BoundedIterator.ext_pos_iff, reaches.toString.symm, bit₀.toEnd_pos, bit.pos_eq_of_not_hasNext hnext]
+      subst bit
+      intro ⟨bit, update, reaches, path⟩
+      have between : bit.BetweenI bit₀ bit₀.toEnd := ⟨reaches, reaches.reaches_toEnd_of_reaches⟩
+      simp [BoundedIterator.BetweenI.iffE] at between
+      match between with
+      | .inl between => exact .inl ⟨bit, update, between, path⟩
+      | .inr ⟨_, eq⟩ => exact .inr ⟨update, eq ▸ path⟩
 
 end captureNext.go
 
